\begin{flalign*}
&\rho = \lambda \frac{\E S}{c} \\
&\E{W_Q} = \frac{C_a^2 + C_s^2}{2} \frac{\rho^{\sqrt{2(c+1)}-1}}{c(1-\rho)} \E S  \\
&\text{Batching: } C_{sB}^2 = \frac{B \V{S_0}+\V{T}}{(B\E{S_0}+\E{T})^2} \\ 
&\text{Nonpreemptive: } \V{S} = \V{S_0} + \frac{\V{T}}{B} + \frac{B -1}{B^2}(\E{T})^2\\
&\text{Preemptive: } A = \frac{m_f}{m_r+m_f}, C_s^2 = C_0^2 + 2A(1-A)\frac{m_r}{\E{S_0}} \\
%& \sigma_s^2 = \sigma_0^2 + \sigma_r^2 f_r + f_r(1-f_r)(\E{S_r})^2 
\\
& C_{di}^2 = 1 + (1-\rho_i^2)(C_{ai}^2 - 1) + \frac{\rho_i^2}{\sqrt{c_i}}(C_{si}^2-1) 
 &\quad 
%C_{ij}^2 = P_{ij}C_{di}^2 + 1 - P_{ij}
\\
& f_i(n_i) = 
            \begin{cases}
              G(i)^{-1} (c_i\rho_i)^{n_i}(n_i!)^{-1}, &\text{ if } n_i < c_i, \\ 
              G(i)^{-1} c_i^{c_i}\rho_i^{n_i}(c_i!)^{-1}, &\text{ if } n_i \geq c_i \\ 
            \end{cases} \\
&\quad \text{with } G(i) = \sum_{n=0}^{c_i-1} \frac{(c_i\rho_i)^n}{n!} + \frac{(c_i\rho_i)^{c_i}}{c_i!}\frac{1}{1-\rho_i} \\
& \E{L_i} = \frac{(c_i\rho_i)^{c_i}}{c_i!G(i)}\frac{\rho_i}{(1-\rho_i)^2} + c_i \rho_i &\quad
% C_{si}^2 = \max\{C_{si}^2, 0.2\} 
\\
%& Q_{ij} = \frac{\lambda_{ij}}{\lambda_j}, i=0\ldots M, j=1\ldots M &\quad C_{aj}^2 = w_j\sum_{i=0}^M Q_{ij}C_{ij}^2 + 1 - w_j \\
%& w_j = (1+4(1-\rho_j)^2(v_j-1))^{-1} &\quad 
% v_j = \left(\sum_{i=0}^M Q_{ij}^2\right)^{-1}, \, j=1,\ldots, M,\\
& f_{i}(n_i) = \frac{1}{\Pi_{k=1}^{n_i} \min\{k, c_i\}}\left(\frac{V_i}{\mu_i}\right)^{n_i}, i=0\ldots M \\
& V_i = (V P)_i = \sum_{j=0}^M V_j P_{ji}\\
%& G(m,n) = \sum_{k=0}^n f_m(k) G(m-1, n-k) &\quad  G(m,0) = 1, G(0,n) = \mu_0^{-n}, \\
%& \E{W_j(n)} = \E{L_j(n-1) + 1} \E{S_j} &\quad \E{L_j(n)} = \TH_j(n) \E{W_j(n)} \\
%& \TH_0(n) = \frac{n}{\sum_{j=0}^M V_j \E{W_j(n)}}  &\quad  \TH_j(n) = V_j \TH_0(n) \\
%&  p_j(0|0) = 1  &\quad \E{W_j(n)} = \sum_{k=c_j}^{n-1} \frac{k-c_j+1}{c_j \mu_j} p_j(k|n-1) + \frac{1}{\mu_j} \\
%& p_j(k|n) = \frac{\TH_j(n)}{\mu_j \min\{c_j,k\}} p_j(k-1|n-1), k=1\ldots N &\quad p_j(0|n) = 1 - \sum_{k=1}^n p_j(k|n).
\end{flalign*}


